\begin{theorem}[Cyclics between consecutive squares (resolves Conj.~9 of \cite{Cohen2025})]\label{thm:squares}
As $n\to\infty$,
\[
 C\big((n+1)^2\big) - C(n^2) \sim \frac{2n}{e^{\gamma}\,\log_3 n}\left(1-\frac{\gamma}{\log_3 n}\right).
\]
\end{theorem}

\begin{proof}
Write $L(x):=\log_3 x$ and recall Pollack's asymptotic expansion (as $x\to\infty$), with remainder term uniform when comparing $x$ and $\lambda x$ for fixed $\lambda$ in compact subsets of $(0,\infty)$ (which is all we use below):
\[
 C(x)=e^{-\gamma}x\Big(\frac{1}{L(x)}-\frac{\gamma}{L(x)^2}+O\Big(\frac{1}{L(x)^3}\Big)\Big).
\]
Set
\[
 \ell_1(x):=e^{-\gamma}\Big(\frac{1}{L(x)}-\frac{\gamma}{L(x)^2}\Big),\qquad a(x):=x\,\ell_1(x).
\]
For later reference we record the auxiliary function explicitly:
\begin{equation}\label{eq:aux-a}
 \boxed{\ a(x)\ :=\ e^{-\gamma}\,x\Big(\frac{1}{\log_3 x}-\frac{\gamma}{\log_3^2 x}\Big)\ }.
\end{equation}
We first prove the fixed-scale increment asymptotic; throughout, the $O(\cdot)$ bounds from Pollack's expansion are uniform for $\lambda$ in compact subsets of $(0,\infty)$, since we only compare $x$ and $\lambda x$ with $\lambda$ fixed.

\textit{Lemma (uniform increment).} For each fixed $\lambda>0$,
\[
 \frac{C(\lambda x)-C(x)}{a(x)(\lambda-1)}\;\longrightarrow\;1\qquad (x\to\infty),
\]
uniformly for $\lambda$ in compact subsets of $(0,\infty)$.

\textit{Proof.} Write $L:=L(x)$ and $L_\lambda:=L(\lambda x)$. Then
\[
 C(\lambda x)-C(x)
 =e^{-\gamma}x\Big(\lambda\Big(\frac{1}{L_\lambda}-\frac{\gamma}{L_\lambda^2}\Big)
 -\Big(\frac{1}{L}-\frac{\gamma}{L^2}\Big)\Big)\;+
 \;O\Big(\frac{x}{L^3}\Big).
\]
Set $f(u):=u^{-1}-\gamma u^{-2}$. Then
\[
 \lambda f(L_\lambda)-f(L)=(\lambda-1)f(L)+\lambda\bigl(f(L_\lambda)-f(L)\bigr).
\]
To handle $L_\lambda-L$, note that with $\log_1 x=\log x$ and $\log_2 x=\log\log x$,
\[
 L_\lambda-L
 =\log\Bigl(1+\frac{\log\bigl(1+\tfrac{\log\lambda}{\log x}\bigr)}{\log_2 x}\Bigr)
 =:\Delta.
\]
Since $\lambda$ is fixed, $\log\lambda$ is constant and hence
\[
 \Delta=O\!\Big(\frac{1}{\log x\,\log_2 x}\Big).
\]
By Taylor's theorem,
\[
 f(L_\lambda)-f(L)=f'(L)\,\Delta+O\Big(\frac{\Delta^2}{L^3}\Big),\qquad f'(L)=-\frac{1}{L^2}+\frac{2\gamma}{L^3}.
\]
Therefore
\[
 C(\lambda x)-C(x)=(\lambda-1)a(x)\;+
 \;e^{-\gamma}x\,\lambda f'(L)\,\Delta
 \;+
 \;O\Big(\frac{x\,\Delta^2}{L^3}\Big)
 \;+
 \;O\Big(\frac{x}{L^3}\Big).
\]
Divide by $a(x)(\lambda-1)=e^{-\gamma}x(\lambda-1)f(L)$. Since $f(L)\asymp 1/L$, $f'(L)=O(1/L^2)$, and $\Delta=O(1/(\log x\,\log_2 x))$, we obtain
\[
 \frac{e^{-\gamma}x\,\lambda f'(L)\,\Delta}{a(x)(\lambda-1)}
 \ll \frac{\Delta}{L}\;=\;O\!\Big(\frac{1}{\log x\,\log_2 x\,L}\Big)\to 0,
\]
while
\[
 \frac{x\,\Delta^2/L^3}{a(x)(\lambda-1)}\ll \frac{\Delta^2}{L^2}\to 0,\qquad
 \frac{x/L^3}{a(x)(\lambda-1)}\ll \frac{1}{L^2}\to 0.
\]
Hence the ratio tends to $1$, proving the lemma. \qed

As a corollary, for fixed $\lambda>0$ one has the drift expansion
\begin{equation}\label{eq:L-drift}
 L(\lambda x)=L(x)+\frac{\log\lambda}{\log_2 x}+O\!\Big(\frac{1}{\log_2^2 x}\Big)\qquad(x\to\infty),
\end{equation}
which is obtained by expanding $\log\bigl(\log(\lambda x)\bigr)$ around $\log x$; we use this below with $\lambda=2$.

By the lemma, $C$ belongs to de Haan's class of $\Pi$-variation of index $1$ with characteristic $\varphi(\lambda)=\lambda-1$ and auxiliary function $a(x)$ (see \cite[\S3.7]{BGT1989}). By Bingham--Goldie--Teugels \cite[Th.~3.7.2]{BGT1989} (local increments for $\Pi$-variation), we then have
\[
 C(x+h)-C(x)\sim a(x)\,\varphi\!\Big(1+\frac{h}{x}\Big)\sim a(x)\,\frac{h}{x}
 \qquad (x\to\infty),\quad h=o(x),
\]
using $\varphi'(1)=1$ for the second asymptotic.

Apply this with $x=n^2$ and $h=(n+1)^2-n^2=2n+1\sim 2n$ to get
\[
 C\big((n+1)^2\big)-C(n^2)\sim (2n)\,\ell_1(n^2)
 =(2n)\,e^{-\gamma}\Big(\frac{1}{L(n^2)}-\frac{\gamma}{L(n^2)^2}\Big).
\]
Now set $L:=\log_3 n$. Then
\[
 L(n^2)=\log_3(n^2)=\log\bigl(\log(2\log n)\bigr)=\log\bigl(\log_2 n+\log 2\bigr)
 = L + \delta,
\]
where
\[
 \delta=\log\Bigl(1+\frac{\log 2}{\log_2 n}\Bigr)=O\!\Big(\frac{1}{\log_2 n}\Big)
 \ =\ \frac{\log 2}{\log_2 n}+O\!\Big(\frac{1}{\log_2^2 n}\Big)\qquad\text{(by \eqref{eq:L-drift} with $\lambda=2$).}
\]
Write $\ell_1(n^2)=e^{-\gamma}f(L(n^2))$ with $f(u)=u^{-1}-\gamma u^{-2}$. Since $f'(u)=-u^{-2}+2\gamma u^{-3}=O(1/u^2)$, the mean value theorem gives
\[
 \ell_1(n^2)=e^{-\gamma}\Big(f(L)+O\Big(\frac{\delta}{L^2}\Big)\Big)
 =e^{-\gamma}\Big(\frac{1}{L}-\frac{\gamma}{L^2}\Big)\Big(1+O\Big(\frac{\delta}{L}\Big)\Big).
\]
Because $\delta/L=O\big(1/(\log_2 n\,\log_3 n)\big)=o(1)$, we may replace $L(n^2)$ by $L=\log_3 n$ inside $\ell_1$ at a relative $o(1)$ cost. Therefore
\[
 C\big((n+1)^2\big)-C(n^2)
 \sim (2n)\,e^{-\gamma}\Big(\frac{1}{\log_3 n}-\frac{\gamma}{(\log_3 n)^2}\Big)
 =\frac{2n}{e^{\gamma}\,\log_3 n}\Big(1-\frac{\gamma}{\log_3 n}\Big),
\]
which is exactly the asserted asymptotic.
\end{proof}
